examples/dynamic_isolation/Util.v
@@ -1,0 +1,41 @@
+Require Import Coq.Lists.List.
+Import ListNotations.
+
+Ltac simplify_forall :=
+  match goal with
+  | H: Forall2 _ [] (_ :: _) |- _ => solve[inversion H]
+  | H: Forall2 _ (_ :: _) [] |- _ => solve[inversion H]
+  | H: Forall2 _ [] [] |- _ => solve[constructor]
+  end.
+
+
+Lemma Forall2_eq : forall {A} (xs ys: list A),
+  List.Forall2 (@eq A) xs ys ->
+  xs = ys.
+Proof.
+  induction xs; intros.
+  - destruct ys; intuition; simplify_forall.
+  - destruct ys; simpl in *; try simplify_forall.
+    f_equal.
+    + inversion H; auto.
+    + apply IHxs; inversion H; auto.
+Qed.
+
+Lemma Forall2_compose : forall {X Y Z} {P: X -> Y -> Prop} {Q: Y -> Z -> Prop} {R: X -> Z -> Prop}
+                          {xs: list X} {ys: list Y} {zs: list Z},
+  (forall x y z, P x y -> Q y z -> R x z) ->
+  List.Forall2 P xs ys ->
+  List.Forall2 Q ys zs ->
+  List.Forall2 R xs zs.
+Proof.
+  induction xs.
+  - induction ys; induction zs; intuition; simplify_forall.
+  - induction ys; intuition; try simplify_forall.
+    generalize dependent zs.
+    induction zs; intuition; try simplify_forall.
+    inversion_clear H0; subst.
+    inversion_clear H1; subst.
+    constructor.
+    + eapply H; eauto.
+    + eapply IHxs; eauto.
+Qed.
